%2multibyte Version: 5.50.0.2960 CodePage: 1252

\documentclass[11pt]{article}

\usepackage{amssymb}
\usepackage{graphicx}
\usepackage{amsmath}
\usepackage{lineno}
\usepackage{fancybox}
\usepackage{fancyhdr}
\usepackage{rotating}
\usepackage{sectsty}

\setcounter{MaxMatrixCols}{10}

\begin{document}

\section{Appendix}

Letting $\eta _{t}^{s}$ , $\eta _{t}^{k}$ and $\lambda _{t}$ be the
Lagrangian multipliers on equations (\ref{3}), (\ref{4}) and (\ref{6})
respectively, the first order conditions are given by:

\begin{equation}
c_{t}:[c_{t}-\varkappa c_{t-1}]^{-\gamma }-\varkappa \beta (1+\mathfrak{g}%
)[c_{t+1}-\varkappa c_{t}]^{-\gamma }=\lambda _{t},  \label{A1}
\end{equation}

\begin{equation}
g_{t}:[g_{t}-\varkappa g_{t-1}]^{-\gamma }-\varkappa \beta (1+\mathfrak{g}%
)[g_{t+1}-\varkappa g_{t}]^{-\gamma }=\lambda _{t},
\end{equation}

\begin{equation}
i_{t}^{k}:e_{k}\eta _{t}^{k}=\lambda _{t},  \label{A3}
\end{equation}

\begin{equation}
i_{t}^{s}:e_{s}\eta _{t}^{s}=\lambda _{t},  \label{A4}
\end{equation}

\begin{equation}
d_{t}:\lambda _{t}=\beta \lambda _{t+1}\left\{ 
\begin{array}{c}
1+r^{\ast }+\frac{\pi }{\rho _{1}^{2}}\left[ \exp \left[ \rho _{1}(d_{t}-%
\bar{d}-\psi V_{t})\right] -\rho _{2}(d_{t}-\overline{d}-\psi V_{t})-\rho
_{3}\right] \\ 
+\frac{\pi }{\rho _{1}^{2}}\left[ \rho _{1}\exp \left[ \rho _{1}(d_{t}-\bar{d%
}-\psi V_{t})\right] -\rho _{2}\right] d_{t}%
\end{array}%
\right\} ,  \label{A5}
\end{equation}

\begin{equation}
k_{t}:\lambda _{t}=\beta (1+\mathfrak{g})\lambda _{t+1}\frac{\left[
e_{k}\theta _{k}\frac{y_{t+1}^{n}}{k_{t}}+(1-\delta _{k})-e_{k}\frac{\phi
_{k}}{2}\left( \frac{k_{t+1}}{k_{t}}-1\right) ^{2}+e_{k}\phi _{k}\left( 
\frac{k_{t+1}}{k_{t}}-1\right) \frac{k_{t+1}}{k_{t}}\right] }{\left[ (1+%
\mathfrak{g})+e_{k}\phi _{k}\left( \frac{k_{t}}{k_{t-1}}-1\right) \right] },
\label{A6}
\end{equation}

\begin{equation}
s_{t}:\lambda _{t}=\beta (1+\mathfrak{g})\lambda _{t+1}\frac{\left[
e_{s}\theta _{s}\frac{y_{t+1}^{n}}{s_{t}}+(1-\delta _{s})-e_{s}\frac{\phi
_{s}}{2}\left( \frac{s_{t+1}}{s_{t}}-1\right) ^{2}+e_{s}\phi _{s}\left( 
\frac{s_{t+1}}{s_{t}}-1\right) \frac{s_{t+1}}{s_{t}}\right] }{\left[ (1+%
\mathfrak{g})+e_{s}\phi _{s}\left( \frac{s_{t}}{s_{t-1}}-1\right) \right] },
\label{A7}
\end{equation}

\begin{equation}
\eta _{t}^{s}:(1+\mathfrak{g})s_{t+1}=e_{s}i_{t}^{s}+(1-\delta _{s})s_{t},
\label{A8}
\end{equation}

\begin{equation}
\eta _{t}^{k}:(1+\mathfrak{g})k_{t+1}=e_{k}i_{t}^{k}+(1-\delta _{k})k_{t},
\label{A9}
\end{equation}

\begin{equation}
\lambda _{t}:(1+\mathfrak{g}%
)d_{t}=(1+r_{t-1})d_{t-1}+c_{t}+i_{t}^{k}+AC_{t}^{k}+g_{t}+i_{t}^{s}+AC_{t}^{s}-y_{t}^{n}-y_{t}^{o}-T_{t}.
\label{A10}
\end{equation}

At steady-state, we find that:

\begin{equation}
\lbrack c(1-\varkappa )]^{-\gamma }[1-\varkappa \beta (1+\mathfrak{g}%
)]=\lambda ,  \label{SS1}
\end{equation}

\begin{equation}
\kappa \lbrack g(1-\varkappa )]^{-\gamma }[1-\varkappa \beta (1+\mathfrak{g}%
)]=\lambda ,  \label{SS2}
\end{equation}

\begin{equation}
e_{k}\eta ^{k}=\lambda ,  \label{SS3}
\end{equation}

\begin{equation}
e_{s}\eta ^{s}=\lambda ,  \label{SS4}
\end{equation}

\begin{equation}
1=\beta \left[ 1+r^{\ast }+\frac{\pi }{\rho _{1}^{2}}[1-\rho _{3}+(\rho
_{1}-\rho _{2})d]\right] ,  \label{SS5}
\end{equation}

\begin{equation}
1=\beta \left[ e_{k}\theta _{k}\frac{y^{n}}{k}+(1-\delta _{k})\right] ,
\label{SS6}
\end{equation}

\begin{equation}
1=\beta \left[ e_{s}\theta _{s}\frac{y^{n}}{s}+(1-\delta _{s})\right] ,
\label{SS7}
\end{equation}

\begin{equation}
s(\mathfrak{g}+\delta _{s})=e_{s}i^{s},  \label{SS8}
\end{equation}

\begin{equation}
k(\mathfrak{g}+\delta _{k})=e_{k}i^{k},  \label{SS9}
\end{equation}

\begin{equation}
(\mathfrak{g}-r)d+y^{n}+y^{o}+T=c+i^{k}+g+i^{s}.  \label{SS10}
\end{equation}

Combining (\ref{SS1}) and (\ref{SS2}):

\begin{equation}
\kappa =\left( \frac{g}{c}\right) ^{\gamma }  \label{SS11}
\end{equation}

\end{document}
